updated Eisbach, using version 5df3d8c72403 of its Bitbucket repository;

src/HOL/Eisbach/Tests.thy
@@ -8,12 +8,12 @@ theory Tests
 imports Main Eisbach_Tools
 begin
 
+
 section \<open>Named Theorems Tests\<close>
 
 named_theorems foo
 
-method foo declares foo =
-  \<open>rule foo\<close>
+method foo declares foo = (rule foo)
 
 lemma
   assumes A [foo]: A
@@ -30,12 +30,12 @@ begin
 
   fix A y
   have "(\<And>x. A x) \<Longrightarrow> A y"
-    apply (rule dup, match prems in Y: "\<And>B. P B" for P \<Rightarrow> \<open>match (P) in A \<Rightarrow> \<open>print_fact Y, rule Y\<close>\<close>)
-    apply (rule dup, match prems in Y: "\<And>B :: 'a. P B" for P \<Rightarrow> \<open>match (P) in A \<Rightarrow> \<open>print_fact Y, rule Y\<close>\<close>)
-    apply (rule dup, match prems in Y: "\<And>B :: 'a. P B" for P \<Rightarrow> \<open>match concl in "P y" for y \<Rightarrow> \<open>print_fact Y, print_term y, rule Y[where B=y]\<close>\<close>)
-    apply (rule dup, match prems in Y: "\<And>B :: 'a. P B" for P \<Rightarrow> \<open>match concl in "P z" for z \<Rightarrow> \<open>print_fact Y, print_term y, rule Y[where B=z]\<close>\<close>)
-    apply (rule dup, match concl in "P y" for P \<Rightarrow> \<open>match prems in Y: "\<And>z. P z" \<Rightarrow> \<open>print_fact Y, rule Y[where z=y]\<close>\<close>)
-    apply (match prems in Y: "\<And>z :: 'a. P z" for P \<Rightarrow> \<open>match concl in "P y" \<Rightarrow> \<open>print_fact Y, rule Y[where z=y]\<close>\<close>)
+    apply (rule dup, match premises in Y: "\<And>B. P B" for P \<Rightarrow> \<open>match (P) in A \<Rightarrow> \<open>print_fact Y, rule Y\<close>\<close>)
+    apply (rule dup, match premises in Y: "\<And>B :: 'a. P B" for P \<Rightarrow> \<open>match (P) in A \<Rightarrow> \<open>print_fact Y, rule Y\<close>\<close>)
+    apply (rule dup, match premises in Y: "\<And>B :: 'a. P B" for P \<Rightarrow> \<open>match conclusion in "P y" for y \<Rightarrow> \<open>print_fact Y, print_term y, rule Y[where B=y]\<close>\<close>)
+    apply (rule dup, match premises in Y: "\<And>B :: 'a. P B" for P \<Rightarrow> \<open>match conclusion in "P z" for z \<Rightarrow> \<open>print_fact Y, print_term y, rule Y[where B=z]\<close>\<close>)
+    apply (rule dup, match conclusion in "P y" for P \<Rightarrow> \<open>match premises in Y: "\<And>z. P z" \<Rightarrow> \<open>print_fact Y, rule Y[where z=y]\<close>\<close>)
+    apply (match premises in Y: "\<And>z :: 'a. P z" for P \<Rightarrow> \<open>match conclusion in "P y" \<Rightarrow> \<open>print_fact Y, rule Y[where z=y]\<close>\<close>)
     done
 
   assume X: "\<And>x. A x" "A y"
@@ -44,37 +44,48 @@ begin
     apply (match X in Y:"B ?x" and Y':"B ?x" for B \<Rightarrow> \<open>print_fact Y, print_term B\<close>)
     apply (match X in Y:"B x" and Y':"B x" for B x \<Rightarrow> \<open>print_fact Y, print_term B, print_term x\<close>)
     apply (insert X)
-    apply (match prems in Y:"\<And>B. A B" and Y':"B y" for B and y :: 'a \<Rightarrow> \<open>print_fact Y[where B=y], print_term B\<close>)
-    apply (match prems in Y:"B ?x" and Y':"B ?x" for B \<Rightarrow> \<open>print_fact Y, print_term B\<close>)
-    apply (match prems in Y:"B x" and Y':"B x" for B x \<Rightarrow> \<open>print_fact Y, print_term B\<close>)
-    apply (match concl in "P x" and "P y" for P x \<Rightarrow> \<open>print_term P, print_term x\<close>)
+    apply (match premises in Y:"\<And>B. A B" and Y':"B y" for B and y :: 'a \<Rightarrow> \<open>print_fact Y[where B=y], print_term B\<close>)
+    apply (match premises in Y:"B ?x" and Y':"B ?x" for B \<Rightarrow> \<open>print_fact Y, print_term B\<close>)
+    apply (match premises in Y:"B x" and Y':"B x" for B x \<Rightarrow> \<open>print_fact Y, print_term B\<close>)
+    apply (match conclusion in "P x" and "P y" for P x \<Rightarrow> \<open>print_term P, print_term x\<close>)
     apply assumption
     done
+
+  {
+   fix B x y
+   assume X: "\<And>x y. B x x y"
+   have "B x x y"
+     by (match X in Y:"\<And>y. B y y z" for z \<Rightarrow> \<open>rule Y[where y=x]\<close>)
+
+   fix A B
+   have "(\<And>x y. A (B x) y) \<Longrightarrow> A (B x) y"
+     by (match premises in Y: "\<And>xx. ?H (B xx)" \<Rightarrow> \<open>rule Y\<close>)
+  }
 
   (* match focusing retains prems *)
   fix B x
   have "(\<And>x. A x) \<Longrightarrow> (\<And>z. B z) \<Longrightarrow> A y \<Longrightarrow> B x"
-    apply (match prems in Y: "\<And>z :: 'a. A z"  \<Rightarrow> \<open>match prems in Y': "\<And>z :: 'b. B z" \<Rightarrow> \<open>print_fact Y, print_fact Y', rule Y'[where z=x]\<close>\<close>)
+    apply (match premises in Y: "\<And>z :: 'a. A z"  \<Rightarrow> \<open>match premises in Y': "\<And>z :: 'b. B z" \<Rightarrow> \<open>print_fact Y, print_fact Y', rule Y'[where z=x]\<close>\<close>)
     done
 
   (*Attributes *)
   fix C
   have "(\<And>x :: 'a. A x)  \<Longrightarrow> (\<And>z. B z) \<Longrightarrow> A y \<Longrightarrow> B x \<and> B x \<and> A y"
     apply (intro conjI)
-    apply (match prems in Y: "\<And>z :: 'a. A z" and Y'[intro]:"\<And>z :: 'b. B z" \<Rightarrow> \<open>fastforce\<close>)
-    apply (match prems in Y: "\<And>z :: 'a. A z"  \<Rightarrow> \<open>match prems in Y'[intro]:"\<And>z :: 'b. B z" \<Rightarrow> \<open>fastforce\<close>\<close>)
-    apply (match prems in Y[thin]: "\<And>z :: 'a. A z"  \<Rightarrow> \<open>(match prems in Y':"\<And>z :: 'a. A z" \<Rightarrow> \<open>fail\<close> \<bar> Y': "?H" \<Rightarrow> \<open>-\<close>)\<close>)
+    apply (match premises in Y: "\<And>z :: 'a. A z" and Y'[intro]:"\<And>z :: 'b. B z" \<Rightarrow> \<open>fastforce\<close>)
+    apply (match premises in Y: "\<And>z :: 'a. A z"  \<Rightarrow> \<open>match premises in Y'[intro]:"\<And>z :: 'b. B z" \<Rightarrow> \<open>fastforce\<close>\<close>)
+    apply (match premises in Y[thin]: "\<And>z :: 'a. A z"  \<Rightarrow> \<open>(match premises in Y':"\<And>z :: 'a. A z" \<Rightarrow> \<open>print_fact Y,fail\<close> \<bar> Y': "?H" \<Rightarrow> \<open>-\<close>)\<close>)
     apply assumption
     done
 
   fix A B C D
   have "\<And>uu'' uu''' uu uu'. (\<And>x :: 'a. A uu' x)  \<Longrightarrow> D uu y \<Longrightarrow> (\<And>z. B uu z) \<Longrightarrow> C uu y \<Longrightarrow> (\<And>z y. C uu z)  \<Longrightarrow> B uu x \<and> B uu x \<and> C uu y"
-    apply (match prems in Y[thin]: "\<And>z :: 'a. A ?zz' z" and
+    apply (match premises in Y[thin]: "\<And>z :: 'a. A ?zz' z" and
                           Y'[thin]: "\<And>rr :: 'b. B ?zz rr" \<Rightarrow>
           \<open>print_fact Y, print_fact Y', intro conjI, rule Y', insert Y', insert Y'[where rr=x]\<close>)
-    apply (match prems in Y:"B ?u ?x" \<Rightarrow> \<open>rule Y\<close>)
+    apply (match premises in Y:"B ?u ?x" \<Rightarrow> \<open>rule Y\<close>)
     apply (insert TrueI)
-    apply (match prems in Y'[thin]: "\<And>ff. B uu ff" for uu \<Rightarrow> \<open>insert Y', drule meta_spec[where x=x]\<close>)
+    apply (match premises in Y'[thin]: "\<And>ff. B uu ff" for uu \<Rightarrow> \<open>insert Y', drule meta_spec[where x=x]\<close>)
     apply assumption
     done
 
@@ -82,33 +93,33 @@ begin
   (* Multi-matches. As many facts as match are bound. *)
   fix A B C x
   have "(\<And>x :: 'a. A x) \<Longrightarrow> (\<And>y :: 'a. B y) \<Longrightarrow> C y \<Longrightarrow> (A x \<and> B y \<and> C y)"
-    apply (match prems in Y[thin]: "\<And>z :: 'a. ?A z" (multi) \<Rightarrow> \<open>intro conjI, (rule Y)+\<close>)
-    apply (match prems in Y[thin]: "\<And>z :: 'a. ?A z" (multi) \<Rightarrow> \<open>fail\<close> \<bar> "C y" \<Rightarrow> \<open>-\<close>) (* multi-match must bind something *)
-    apply (match prems in Y: "C y" \<Rightarrow> \<open>rule Y\<close>)
+    apply (match premises in Y[thin]: "\<And>z :: 'a. ?A z" (multi) \<Rightarrow> \<open>intro conjI, (rule Y)+\<close>)
+    apply (match premises in Y[thin]: "\<And>z :: 'a. ?A z" (multi) \<Rightarrow> \<open>fail\<close> \<bar> "C y" \<Rightarrow> \<open>-\<close>) (* multi-match must bind something *)
+    apply (match premises in Y: "C y" \<Rightarrow> \<open>rule Y\<close>)
     done
 
   fix A B C x
   have "(\<And>x :: 'a. A x) \<Longrightarrow> (\<And>y :: 'a. B y) \<Longrightarrow> C y \<Longrightarrow> (A x \<and> B y \<and> C y)"
-    apply (match prems in Y[thin]: "\<And>z. ?A z" (multi) \<Rightarrow> \<open>intro conjI, (rule Y)+\<close>)
-    apply (match prems in Y[thin]: "\<And>z. ?A z" (multi) \<Rightarrow> \<open>fail\<close> \<bar> "C y" \<Rightarrow> \<open>-\<close>) (* multi-match must bind something *)
-    apply (match prems in Y: "C y" \<Rightarrow> \<open>rule Y\<close>)
+    apply (match premises in Y[thin]: "\<And>z. ?A z" (multi) \<Rightarrow> \<open>intro conjI, (rule Y)+\<close>)
+    apply (match premises in Y[thin]: "\<And>z. ?A z" (multi) \<Rightarrow> \<open>fail\<close> \<bar> "C y" \<Rightarrow> \<open>-\<close>) (* multi-match must bind something *)
+    apply (match premises in Y: "C y" \<Rightarrow> \<open>rule Y\<close>)
     done
 
 
   (*We may use for-fixes in multi-matches too. All bound facts must agree on the fixed term *)
   fix A B C x
   have "(\<And>y :: 'a. B y \<and> C y) \<Longrightarrow> (\<And>x :: 'a. A x \<and> B x) \<Longrightarrow> (\<And>y :: 'a. A y \<and> C y) \<Longrightarrow> C y \<Longrightarrow> (A x \<and> B y \<and> C y)"
-    apply (match prems in Y: "\<And>x :: 'a. P x \<and> ?U x" (multi) for P \<Rightarrow> \<open>intro conjI Y[THEN conjunct1]\<close>)
-    apply (match prems in Y: "\<And>z :: 'a. ?A z \<longrightarrow> False" (multi) \<Rightarrow> \<open>print_fact Y, fail\<close> \<bar> "C y" \<Rightarrow> \<open>print_term C\<close>) (* multi-match must bind something *)
-    apply (match prems in Y: "\<And>x. B x \<and> C x" \<Rightarrow> \<open>intro conjI Y[THEN conjunct1]\<close>)
-    apply (match prems in Y: "C ?x" \<Rightarrow> \<open>rule Y\<close>)
+    apply (match premises in Y: "\<And>x :: 'a. P x \<and> ?U x" (multi) for P \<Rightarrow> \<open>intro conjI Y[THEN conjunct1]\<close>)
+    apply (match premises in Y: "\<And>z :: 'a. ?A z \<longrightarrow> False" (multi) \<Rightarrow> \<open>print_fact Y, fail\<close> \<bar> "C y" \<Rightarrow> \<open>print_term C\<close>) (* multi-match must bind something *)
+    apply (match premises in Y: "\<And>x. B x \<and> C x" \<Rightarrow> \<open>intro conjI Y[THEN conjunct1]\<close>)
+    apply (match premises in Y: "C ?x" \<Rightarrow> \<open>rule Y\<close>)
     done
 
   (* Attributes *)
   fix A B C x
   have "(\<And>x :: 'a. A x \<and> B x) \<Longrightarrow> (\<And>y :: 'a. A y \<and> C y) \<Longrightarrow> (\<And>y :: 'a. B y \<and> C y) \<Longrightarrow> C y \<Longrightarrow> (A x \<and> B y \<and> C y)"
-    apply (match prems in Y: "\<And>x :: 'a. P x \<and> ?U x" (multi) for P \<Rightarrow> \<open>match Y[THEN conjunct1]  in Y':"?H"  (multi) \<Rightarrow> \<open>intro conjI,rule Y'\<close>\<close>)
-    apply (match prems in Y: "\<And>x :: 'a. P x \<and> ?U x" (multi) for P \<Rightarrow> \<open>match Y[THEN conjunct2]  in Y':"?H"  (multi) \<Rightarrow> \<open>rule Y'\<close>\<close>)
+    apply (match premises in Y: "\<And>x :: 'a. P x \<and> ?U x" (multi) for P \<Rightarrow> \<open>match Y[THEN conjunct1]  in Y':"?H"  (multi) \<Rightarrow> \<open>intro conjI,rule Y'\<close>\<close>)
+    apply (match premises in Y: "\<And>x :: 'a. P x \<and> ?U x" (multi) for P \<Rightarrow> \<open>match Y[THEN conjunct2]  in Y':"?H"  (multi) \<Rightarrow> \<open>rule Y'\<close>\<close>)
     apply assumption
     done
 
@@ -123,19 +134,30 @@ begin
   (* Testing THEN_ALL_NEW within match *)
   fix A B C x
   have "(\<And>x :: 'a. A x \<and> B x) \<Longrightarrow> (\<And>y :: 'a. A y \<and> C y) \<Longrightarrow> (\<And>y :: 'a. B y \<and> C y) \<Longrightarrow> C y \<Longrightarrow> (A x \<and> B y \<and> C y)"
-    apply (match prems in Y: "\<And>x :: 'a. P x \<and> ?U x" (multi) for P \<Rightarrow> \<open>intro conjI ; ((rule Y[THEN conjunct1])?); rule Y[THEN conjunct2] \<close>)
+    apply (match premises in Y: "\<And>x :: 'a. P x \<and> ?U x" (multi) for P \<Rightarrow> \<open>intro conjI ; ((rule Y[THEN conjunct1])?); rule Y[THEN conjunct2] \<close>)
     done
 
   (* Cut tests *)
   fix A B C
 
   have "D \<and> C  \<Longrightarrow> A \<and> B  \<Longrightarrow> A \<longrightarrow> C \<Longrightarrow> D \<longrightarrow> True \<Longrightarrow> C"
-    by (((match prems in I: "P \<and> Q" (cut)
+    by (((match premises in I: "P \<and> Q" (cut)
               and I': "P \<longrightarrow> ?U" for P Q \<Rightarrow> \<open>rule mp [OF I' I[THEN conjunct1]]\<close>)?), simp)
 
   have "A \<and> B \<Longrightarrow> A \<longrightarrow> C \<Longrightarrow> C"
-    by (((match prems in I: "P \<and> Q" (cut)
+    by (((match premises in I: "P \<and> Q" (cut)
               and I': "P \<longrightarrow> ?U" for P Q \<Rightarrow> \<open>rule mp [OF I' I[THEN conjunct1]]\<close>)?, simp) | simp)
+
+  fix f x y
+  have "f x y \<Longrightarrow> f x y"
+    by (match conclusion in "f x y" for f x y  \<Rightarrow> \<open>print_term f\<close>)
+
+  fix A B C
+  assume X: "A \<and> B" "A \<and> C" C
+  have "A \<and> B \<and> C"
+    by (match X in H: "A \<and> ?H" (multi,cut) \<Rightarrow>
+          \<open>match H in "A \<and> C" and "A \<and> B" \<Rightarrow> \<open>fail\<close>\<close>
+        | simp add: X)
 
 end
 
@@ -144,7 +166,7 @@ end
    legitimate pairs.*)
 
 schematic_lemma "?A x \<Longrightarrow> A x"
-  apply (match concl in "H" for H \<Rightarrow> \<open>match concl in Y for Y \<Rightarrow> \<open>print_term Y\<close>\<close>)
+  apply (match conclusion in "H" for H \<Rightarrow> \<open>match conclusion in Y for Y \<Rightarrow> \<open>print_term Y\<close>\<close>)
   apply assumption
   done
 
@@ -171,7 +193,7 @@ ML \<open>
       NONE => ()
     | SOME _ => error "Found internal fact")\<close>
 
-method uses_test\<^sub>1 uses uses_test\<^sub>1_uses = \<open>rule uses_test\<^sub>1_uses\<close>
+method uses_test\<^sub>1 uses uses_test\<^sub>1_uses = (rule uses_test\<^sub>1_uses)
 
 lemma assumes A shows A by (uses_test\<^sub>1 uses_test\<^sub>1_uses: assms)
 
@@ -184,9 +206,9 @@ ML \<open>test_internal_fact @{context} "Tests.uses_test\<^sub>1.uses_test\<^sub
 (* Testing term and fact passing in recursion *)
 
 method recursion_example for x :: bool uses facts =
-  \<open>match (x) in
+  (match (x) in
     "A \<and> B" for A B \<Rightarrow> \<open>(recursion_example A facts: facts, recursion_example B facts: facts)\<close>
-  \<bar> "?H" \<Rightarrow> \<open>match facts in U: "x" \<Rightarrow> \<open>insert U\<close>\<close>\<close>
+  \<bar> "?H" \<Rightarrow> \<open>match facts in U: "x" \<Rightarrow> \<open>insert U\<close>\<close>)
 
 lemma
   assumes asms: "A" "B" "C" "D"
@@ -196,11 +218,11 @@ lemma
   done
 
 (*Method.sections in existing method*)
-method my_simp\<^sub>1 uses my_simp\<^sub>1_facts = \<open>simp add: my_simp\<^sub>1_facts\<close>
+method my_simp\<^sub>1 uses my_simp\<^sub>1_facts = (simp add: my_simp\<^sub>1_facts)
 lemma assumes A shows A by (my_simp\<^sub>1 my_simp\<^sub>1_facts: assms)
 
 (*Method.sections via Eisbach argument parser*)
-method uses_test\<^sub>2 uses uses_test\<^sub>2_uses = \<open>uses_test\<^sub>1 uses_test\<^sub>1_uses: uses_test\<^sub>2_uses\<close>
+method uses_test\<^sub>2 uses uses_test\<^sub>2_uses = (uses_test\<^sub>1 uses_test\<^sub>1_uses: uses_test\<^sub>2_uses)
 lemma assumes A shows A by (uses_test\<^sub>2 uses_test\<^sub>2_uses: assms)
 
 
@@ -208,7 +230,7 @@ subsection \<open>Declaration Tests\<close>
 
 named_theorems declare_facts\<^sub>1
 
-method declares_test\<^sub>1 declares declare_facts\<^sub>1 = \<open>rule declare_facts\<^sub>1\<close>
+method declares_test\<^sub>1 declares declare_facts\<^sub>1 = (rule declare_facts\<^sub>1)
 
 lemma assumes A shows A by (declares_test\<^sub>1 declare_facts\<^sub>1: assms)
 
@@ -218,26 +240,56 @@ lemma assumes A[declare_facts\<^sub>1]: A shows A by declares_test\<^sub>1
 subsection \<open>Rule Instantiation Tests\<close>
 
 method my_allE\<^sub>1 for x :: 'a and P :: "'a \<Rightarrow> bool" =
-  \<open>erule allE [where x = x and P = P]\<close>
+  (erule allE [where x = x and P = P])
 
 lemma "\<forall>x. Q x \<Longrightarrow> Q x" by (my_allE\<^sub>1 x Q)
 
 method my_allE\<^sub>2 for x :: 'a and P :: "'a \<Rightarrow> bool" =
-  \<open>erule allE [of P x]\<close>
+  (erule allE [of P x])
 
 lemma "\<forall>x. Q x \<Longrightarrow> Q x" by (my_allE\<^sub>2 x Q)
 
 method my_allE\<^sub>3 for x :: 'a and P :: "'a \<Rightarrow> bool" =
-  \<open>match allE [where 'a = 'a] in X: "\<And>(x :: 'a) P R. \<forall>x. P x \<Longrightarrow> (P x \<Longrightarrow> R) \<Longrightarrow> R" \<Rightarrow>
-    \<open>erule X [where x = x and P = P]\<close>\<close>
+  (match allE [where 'a = 'a] in X: "\<And>(x :: 'a) P R. \<forall>x. P x \<Longrightarrow> (P x \<Longrightarrow> R) \<Longrightarrow> R" \<Rightarrow>
+    \<open>erule X [where x = x and P = P]\<close>)
 
 lemma "\<forall>x. Q x \<Longrightarrow> Q x" by (my_allE\<^sub>3 x Q)
 
 method my_allE\<^sub>4 for x :: 'a and P :: "'a \<Rightarrow> bool" =
-  \<open>match allE [where 'a = 'a] in X: "\<And>(x :: 'a) P R. \<forall>x. P x \<Longrightarrow> (P x \<Longrightarrow> R) \<Longrightarrow> R" \<Rightarrow>
-    \<open>erule X [of x P]\<close>\<close>
+  (match allE [where 'a = 'a] in X: "\<And>(x :: 'a) P R. \<forall>x. P x \<Longrightarrow> (P x \<Longrightarrow> R) \<Longrightarrow> R" \<Rightarrow>
+    \<open>erule X [of x P]\<close>)
 
 lemma "\<forall>x. Q x \<Longrightarrow> Q x" by (my_allE\<^sub>4 x Q)
+
+
+
+(* Polymorphism test *)
+
+axiomatization foo' :: "'a \<Rightarrow> 'b \<Rightarrow> 'c \<Rightarrow> bool"
+axiomatization where foo'_ax1: "foo' x y z \<Longrightarrow> z \<and> y"
+axiomatization where foo'_ax2: "foo' x y y \<Longrightarrow> x \<and> z"
+
+lemmas my_thms = foo'_ax1 foo'_ax2
+
+definition first_id where "first_id x = x"
+
+lemmas my_thms' = my_thms[of "first_id x" for x]
+
+method print_conclusion = (match conclusion in concl for concl \<Rightarrow> \<open>print_term concl\<close>)
+
+lemma
+  assumes foo: "\<And>x (y :: bool). foo' (A x) B (A x)"
+  shows "\<And>z. A z \<and> B"
+  apply
+    (match conclusion in "f x y" for f y and x :: "'d :: type" \<Rightarrow> \<open>
+      match my_thms' in R:"\<And>(x :: 'f :: type). ?P (first_id x) \<Longrightarrow> ?R"
+                     and R':"\<And>(x :: 'f :: type). ?P' (first_id x) \<Longrightarrow> ?R'" \<Rightarrow> \<open>
+        match (x) in "q :: 'f" for q \<Rightarrow> \<open>
+          rule R[of q,simplified first_id_def],
+          print_conclusion,
+          rule foo
+      \<close>\<close>\<close>)
+  done
 
 
 ML {*
@@ -254,7 +306,7 @@ local_setup \<open>Local_Theory.add_thms_dynamic (@{binding test_dyn}, Data.get)
 
 setup \<open>Context.theory_map (Data.put @{thms TrueI})\<close>
 
-method dynamic_thms_test = \<open>rule test_dyn\<close>
+method dynamic_thms_test = (rule test_dyn)
 
 locale foo =
   fixes A
@@ -268,5 +320,13 @@ local_setup
 lemma A by dynamic_thms_test
 
 end
+
+(* Method name internalization test *)
+
+method test2 = (simp)
+
+method simp = fail
+
+lemma "A \<Longrightarrow> A" by test2
 
 end
